WIP; MapMAproof

theories/iris_system/invariants.v
@@ -8,75 +8,7 @@ Require Export SRF sProp own.
 
 Definition univ_id := positive.
 
-(* TODO - move to another library? *)
-Section univ_id.
-  Fixpoint pos_sup (p i : positive) : bool :=
-    match p, i with
-    | 1, _ => true
-    | p'~0, i'~0 => pos_sup p' i'
-    | p'~1, i'~1 => pos_sup p' i'
-    | _, _ => false
-    end%positive.
-
-  Fixpoint pos_ext_0 (p : positive) : positive :=
-    match p with
-    | 1 => 1~0
-    | p'~0 => (pos_ext_0 p')~0
-    | p'~1 => (pos_ext_0 p')~1
-    end%positive.
-
-  Fixpoint pos_ext_1 (p : positive) : positive :=
-    match p with
-    | 1 => 1~1
-    | p'~0 => (pos_ext_1 p')~0
-    | p'~1 => (pos_ext_1 p')~1
-    end%positive.
-
-  Lemma pos_sup_refl p :
-    pos_sup p p = true.
-  Proof. induction p; s; eauto. Qed.
-
-  Lemma pos_sup_trans p0 p1 p2
-      (EXT1: pos_sup p0 p1 = true)
-      (EXT2: pos_sup p1 p2 = true) :
-    pos_sup p0 p2 = true.
-  Proof. revert_until p0. induction p0; i; destruct p1, p2; ss; eauto. Qed.
-
-  Lemma pos_ext_0_sup_true p : pos_sup p (pos_ext_0 p) = true.
-  Proof. induction p; s; eauto. Qed.
-
-  Lemma pos_ext_1_sup_true p : pos_sup p (pos_ext_1 p) = true.
-  Proof. induction p; s; eauto. Qed.
-
-  Lemma pos_ext_0_sup_false p : pos_sup (pos_ext_0 p) p = false.
-  Proof. induction p; s; eauto. Qed.
-
-  Lemma pos_ext_1_sup_false p : pos_sup (pos_ext_1 p) p = false.
-  Proof. induction p; s; eauto. Qed.
-
-  Lemma pos_ext_0_neq p : p ≠ pos_ext_0 p.
-  Proof. induction p; eauto; ii; depdes H; eauto. Qed.
-
-  Lemma pos_ext_1_neq p : p ≠ pos_ext_1 p.
-  Proof. induction p; eauto; ii; depdes H; eauto. Qed.
-
-  Lemma pos_ext_0_disj p p' (SUP: pos_sup (pos_ext_1 p) p' = true) :
-    pos_sup (pos_ext_0 p) p' = false.
-  Proof. revert p' SUP. induction p; i; destruct p'; ss; eauto. Qed.
-
-  Lemma pos_ext_1_disj p p' (SUP: pos_sup (pos_ext_0 p) p' = true) :
-    pos_sup (pos_ext_1 p) p' = false.
-  Proof. revert p' SUP. induction p; i; destruct p'; ss; eauto. Qed.
-
-  Lemma pos_sup_cases u k
-      (EQ : (k =? u)%positive = false)
-      (SUP0 : pos_sup (pos_ext_0 u) k = false)
-      (SUP1 : pos_sup (pos_ext_1 u) k = false) :
-    pos_sup u k = false.
-  Proof. revert_until u. induction u; i; destruct k; ss; eauto. Qed.
-End univ_id.
-
-Section resources.
+Section invariants.
   Context `{α : SRFCons.t}.
 
   Canonical Structure SynO n : ofe := leibnizO (SRFSyn.t n).
@@ -127,7 +59,7 @@ Section resources.
   Proof. solve_inG. Qed.
   Global Instance invG_subG {α' Σ Γ} : invGΣ α' Σ → invGΓ Γ → invG α' Σ Γ.
   Proof. i; ss. Qed.
-End resources.
+End invariants.
 
 Section predicates.
   Context `{!subG (Γ : HRA) Σ, !invG α Σ Γ}.
@@ -154,10 +86,10 @@ Section predicates.
     own base_γ (ownI_authR u n I).
 
   (* authorative resource for wsats *)
-  Definition wsat_restR u b : ownIRA :=
+  Definition wsat_authR u b : ownIRA :=
     discrete_fun_singleton u
       ((λ n, if (n <? b) then ε else gmap_view_auth (DfracOwn 1) ∅) : discrete_funUR InvSetRA).
-  Definition wsat_rest u b : iProp Σ := own base_γ (wsat_restR u b).
+  Definition wsat_auth u b : iProp Σ := own base_γ (wsat_authR u b).
 
   (* namespaces *)
   Definition ownER (u : univ_id) (E : coPset) : ownERA :=
@@ -307,20 +239,11 @@ End wsat.
 Section wsats.
   Context `{@SRFIntp.t (domain Σ) α, !invG α Σ Γ, !subG Γ Σ}.
   Local Existing Instances invG_Σ invG_Γ invG_I invG_E invG_D.
-
-  (* resources for multiple wsats *)
-  Definition univs_fun {A : univ_id → ucmra} (u : univ_id) (r : ∀ u, A u) : discrete_funUR A :=
-    λ v, if pos_sup u v then r v else ε.
   
   Definition wsats u n E : iProp Σ :=
-    wsat_rest u n ∗ ownE u E ∗ ownD_auth u ∗ [∗ list] n ∈ (seq 0 n), wsat u n.
+    wsat_auth u n ∗ ownE u E ∗ ownD_auth u ∗ [∗ list] n ∈ (seq 0 n), wsat u n.
 
-  Definition univs u : iProp Σ :=
-    own base_γ (univs_fun u ((λ _ _, gmap_view_auth (DfracOwn 1) ∅) : ownIRA)) ∗
-    own base_γ (univs_fun u (λ _, CoPset ⊤) : ownERA) ∗
-    own base_γ (univs_fun u (λ _, ● (GSet ∅)) : ownDRA).
-
-  (* Definition univs u n : iProp Σ :=
+  Definition univs u n : iProp Σ :=
     [∗ list] v ∈ (seq 0 (Pos.to_nat u)), wsats (Pos.of_nat v) n ⊤.
 
   Lemma univs_split ν υ n : (ν < υ)%positive →
@@ -335,7 +258,7 @@ Section wsats.
     rewrite -{2}(Pos2Nat.id ν) -(big_sepL_cons (λ _ ν, wsats (Pos.of_nat ν) n ⊤)).
     rewrite cons_seq; iCombine "H1" "H" as "H"; rewrite -big_sepL_app -seq_app.
     rewrite /univs. eapply eq_ind; first iExact "H"; repeat f_equal; try lia.
-  Qed. *)
+  Qed.
 
   Local Definition uPred_fupd_def u b (E1 E2 : coPset) (P : iProp Σ) : iProp Σ :=
     wsats u b E1 ==∗ (wsats u b E2 ∗ P).
@@ -395,7 +318,7 @@ Notation "P '=|' u ',' n '|={' E '}=∗' Q" := (P -∗ =|u, n|={E, E}=> Q)%I (at
   (* Definition used_worlds u b E : iProp Σ :=
     wsats u b ∗ ownE u E ∗ ownD_auth u ∗ free_universes. *)
   (* Definition closed_universe u b E : iProp Σ :=
-    used_worlds u b E ∗ wsat_rest u b. *)
+    used_worlds u b E ∗ wsat_auth u b. *)
 
   (* Lemma wsats_fold u b :
     wsats u (S b) ⊣⊢ (wsat u b ∗ wsats u b)%I.
@@ -405,9 +328,9 @@ Notation "P '=|' u ',' n '|={' E '}=∗' Q" := (P -∗ =|u, n|={E, E}=> Q)%I (at
   Qed. *)
 
   (* Lemma free_worlds_alloc u (b b' : level) (NIN : b < b') :
-    wsat_rest u b ⊢ wsat_rest u b' ∗ ([∗ list] n ∈ (seq b (b' - b)), wsat u n).
+    wsat_auth u b ⊢ wsat_auth u b' ∗ ([∗ list] n ∈ (seq b (b' - b)), wsat u n).
   Proof.
-    rewrite /wsat_rest /wsat_authR.
+    rewrite /wsat_auth /wsat_authR.
     induction NIN; iIntros "FW".
     { replace (S b - b) with 1 by lia; ss.
       iEval (rewrite (discrete_fun_delete b (λ n, if n <? b then ε else gmap_view_auth (DfracOwn 1) ∅))) in "FW".
@@ -448,7 +371,7 @@ Notation "P '=|' u ',' n '|={' E '}=∗' Q" := (P -∗ =|u, n|={E, E}=> Q)%I (at
   Qed. *)
 
  (* Lemma free_worlds_nin u (b b' : level) (LE : b <= b')
-    : wsat_rest u b ⊢ wsat_rest u b' ∗
+    : wsat_auth u b ⊢ wsat_auth u b' ∗
                       ([∗ list] n ∈ (seq b (b' - b)), wsat u n).
   Proof.
     iIntros "R".
@@ -458,7 +381,7 @@ Notation "P '=|' u ',' n '|={' E '}=∗' Q" := (P -∗ =|u, n|={E, E}=> Q)%I (at
   Qed.
 
   Lemma wsats_allocs u b b':
-    b <= b' -> wsat_rest u b ∗ wsats u b ⊢ wsat_rest u b' ∗ wsats u b'.
+    b <= b' -> wsat_auth u b ∗ wsats u b ⊢ wsat_auth u b' ∗ wsats u b'.
   Proof.
     iIntros (LE) "(AUTH & SAT)".
     iPoseProof ((free_worlds_nin _ _ _ LE) with "AUTH") as "(AUTH & NEW)". iFrame.
@@ -504,9 +427,9 @@ Notation "P '=|' u ',' n '|={' E '}=∗' Q" := (P -∗ =|u, n|={E, E}=> Q)%I (at
             | None => True
             | Some G => (exists i, i ∉ G /\ φ i)
             end)
-    : wsat_rest u b ∗ ownD_auth u ∗ wsats u b ⊢
+    : wsat_auth u b ∗ ownD_auth u ∗ wsats u b ⊢
         |==> ((∃ i, ⌜φ i⌝ ∧ ownI u n i p)
-              ∗ wsat_rest u (S n) ∗ ownD_auth u ∗ (⟦p⟧ -∗ wsats u (S n))).
+              ∗ wsat_auth u (S n) ∗ ownD_auth u ∗ (⟦p⟧ -∗ wsats u (S n))).
   Proof.
     iIntros "(AUTH & D & WSAT)".
     iPoseProof ((wsats_allocs u b (S n)) with "[AUTH WSAT]") as "[AUTH WSAT]". lia. iFrame.
@@ -520,9 +443,9 @@ Notation "P '=|' u ',' n '|={' E '}=∗' Q" := (P -∗ =|u, n|={E, E}=> Q)%I (at
             | None => True
             | Some G => (exists i, i ∉ G /\ φ i)
             end)
-    : wsat_rest u b ∗ ownD_auth u ∗ wsats u b ∗ ⟦p⟧ ⊢
+    : wsat_auth u b ∗ ownD_auth u ∗ wsats u b ∗ ⟦p⟧ ⊢
         |==> ((∃ i, ⌜φ i⌝ ∧ ownI u n i p)
-                ∗ wsat_rest u (S n) ∗ ownD_auth u ∗ wsats u (S n)).
+                ∗ wsat_auth u (S n) ∗ ownD_auth u ∗ wsats u (S n)).
   Proof.
     iIntros "(A & D & W & P)". iMod (wsats_ownI_alloc_ge_gen with "[A D W]") as "(I & A & D & W)".
     1,2 : eauto. iFrame.
@@ -530,10 +453,10 @@ Notation "P '=|' u ',' n '|={' E '}=∗' Q" := (P -∗ =|u, n|={E, E}=> Q)%I (at
   Qed.
 
   Lemma free_worlds_ownI_le u b n i p :
-    ownI u n i p ∗ wsat_rest u b ⊢ ⌜n < b⌝.
+    ownI u n i p ∗ wsat_auth u b ⊢ ⌜n < b⌝.
   Proof.
     iIntros "(I & AUTH)".
-    unfold ownI, wsat_rest, wsat_rest.
+    unfold ownI, wsat_auth, wsat_auth.
     iCombine "AUTH I" as "AUTH".
     iPoseProof (own_valid with "AUTH") as "%WF".
     unfold wsat_authR, ownIR, maps_to_res, maps_to_res_dep in WF.
@@ -580,7 +503,7 @@ Notation "P '=|' u ',' n '|={' E '}=∗' Q" := (P -∗ =|u, n|={E, E}=> Q)%I (at
   Qed. *)
 
   (* Lemma empty_worlds_split eu:
-    empty_universes eu ⊢ wsat_rest eu 0 ∗ wsats eu 0 ∗ ownE eu ⊤ ∗ ownD_auth eu ∗ empty_universes (pos_ext_0 eu) ∗ empty_universes (pos_ext_1 eu).
+    empty_universes eu ⊢ wsat_auth eu 0 ∗ wsats eu 0 ∗ ownE eu ⊤ ∗ ownD_auth eu ∗ empty_universes (pos_ext_0 eu) ∗ empty_universes (pos_ext_1 eu).
   Proof.
     assert (ERA : URA.extends
               ((ownER eu ⊤) ⋅
