examples/map/MapIMproof.v
@@ -320,9 +320,7 @@ Section wctxr.
   Context `{!invG α Σ Γ, !subG Γ Σ, !sinvG Σ Γ α β τ, !MapMGΓ Γ, !memGΓ Γ}.
   Lemma wctxr n SpcMap SpcMem ginv (INCL : ∀ u, spc_incl (MapMS.Spc u n) (SpcMap u)) :
     w_ctx_refines
-      (λ υ, ((MapM.t υ n ginv (SpcMap υ)) ★ (MemA.t ginv SpcMem), MapM.InitCond))
-      (λ _, (MapI.t                       ★ (MemA.t ginv SpcMem), emp%I)).
-  Proof.
-    exists 1; move => u v Huv; eapply main_adequacy, MapIM.sim; apply INCL.
-  Qed.
+      ((λ υ, (MapM.t υ n ginv (SpcMap υ)) ★ (MemA.t ginv SpcMem)), MapM.InitCond)
+      ((λ _, MapI.t                       ★ (MemA.t ginv SpcMem)), emp%I).
+  Proof. exists 1%positive; intros u v Huv; eapply main_adequacy, MapIM.sim; eauto. Qed.
 End wctxr.
