theories/iris_system/syn_invariants.v
@@ -8,13 +8,13 @@ Local Notation level := nat.
 Variant inv_shape : Type :=
 | _ownI (u : univ_id) (i : positive)
 | _ownI_auth (u : univ_id) (keys : gmap positive unit)
-| _wsat_rest (u : univ_id).
+| _wsat_auth (u : univ_id).
 
 Local Definition inv_degree (s : inv_shape) (sProp : Type) : Type :=
   match s with
   | _ownI u i => fin 1
   | _ownI_auth u keys => positive
-  | _wsat_rest u => fin 0
+  | _wsat_auth u => fin 0
   end.
 
 Global Instance inv_syntax : PF.t := {
@@ -29,7 +29,7 @@ Local Definition inv_interp_aux `{!invG α Σ Γ, !subG Γ Σ} n (s : inv_shape)
   match s with
   | _ownI u i => λ syn _, ownI u n i (syn 0%fin)
   | _ownI_auth u keys => λ syn _, ownI_auth u n (map_imap (λ k v, Some (syn k)) keys)
-  | _wsat_rest u => λ _ _, wsat_rest u n
+  | _wsat_auth u => λ _ _, wsat_auth u n
   end.
 
 Global Instance inv_interp `{!invG α Σ Γ, !subG Γ Σ} :
@@ -49,8 +49,8 @@ Section syn_inv.
     ⟨ _ownI u i, λ _, p ⟩.
   Local Definition syn_ownI_auth u n (I : gmap positive (SRFSyn.t n)) : SRFSyn.t n :=
     ⟨ _ownI_auth u (gset_to_gmap tt (dom I)), λ i, or_else (I !! i) emp%SRF⟩.
-  Local Definition syn_wsat_rest u n : SRFSyn.t n :=
-    ⟨ _wsat_rest u, λ e, match e with end ⟩.
+  Local Definition syn_wsat_auth u n : SRFSyn.t n :=
+    ⟨ _wsat_auth u, λ e, match e with end ⟩.
 
   Local Definition syn_ownE (u : univ_id) n (E : coPset) : SRFSyn.t n :=
     <own> base_γ (ownER u E).
@@ -70,7 +70,7 @@ Section syn_inv.
     | S n' => syn_wsat u n' ∗ ⤉ syn_wsats_aux u n'
     end.
   Local Definition syn_wsats u n (E : coPset) : SRFSyn.t n :=
-    syn_wsat_rest u n ∗ syn_ownE u n E ∗ syn_ownD_auth u n ∗ syn_wsats_aux u n.
+    syn_wsat_auth u n ∗ syn_ownE u n E ∗ syn_ownD_auth u n ∗ syn_wsats_aux u n.
 
   (* Interface for the user *)
   Local Definition syn_inv_def (u : univ_id) (n : level) (N : namespace) p :=
